\documentclass{article}
\usepackage[english]{babel}
\usepackage{amsmath, amssymb, amsthm}

\title{Bootcamp : Maths}
\author{Baptiste Rouger}


\begin{document}

    \maketitle

    \tableofcontents

    \newpage

    \section{Session 1}


    \subsection{Calculus}

    Calculus : study of changes.\\

    2 types of calculus : differential and integral calculus.\\

    Differential : distance $\rightarrow$ speed\\
    Integration : speed $\rightarrow$ distance\\

    \subsubsection{Derivative}

    \paragraph{Definition}

    ~\\The derivative is the slope of the tangent line on a point.\\
    \textit{Definition :} The derivative of $f$ at $x_0$ is the slope of the line tangent to the graph of $f$ at $x_0$.\\
    \[ \lim_{\Delta x \to 0}; \frac{f(x_0 + \Delta x) - f(x_0)}{\Delta x} = f'(x_0) \]



    \paragraph{Some derivatives}
    $f(x) = \frac{1}{x} (x>0)  $\\
    $\frac{\Delta f}{\Delta x} =  \frac{\frac{1}{x_0 + \Delta x} - \frac{1}{x_0}}{\Delta x} = -\frac{1}{x_0^2 + x_0 \Delta x} $
    \[ f'(x_0) = \lim_{\Delta x \to 0}; -\frac{1}{x_0^2 + x_0 \Delta x} = -\frac{1}{x_0^2} \]
    ~\\~\\

    $f(x) = x^n$\\
    \[f'(x) = \lim_{\Delta x \to 0}; \frac{(x + \Delta x)^n - x^n}{\Delta x} = \lim_{\Delta x \to 0}; \frac{(\binom n0 x^n \Delta x ^0 + \binom n1 x^n \Delta x ^1 +... ) - x^n}{\Delta x} = nx^{n-1} \]

    ~\\
    $(f+g)'(x) = f'(x)+g'(x)$


    \paragraph{Continuity}
    ~\\
    Notations : $f'(x) = \frac{dy}{dx} = \frac{df}{dx} = Df = \frac{d}{dx}f$ = y'\\

    \noindent \textit{Example : } 400 ft , $y = 400 - 16t^2$\\
    $400 -16t^2 = 0$\\
    $t = 5$\\
    On average, -80 ft per second. But we want to know the instantaneous speed when the pumpkin hits the ground :\\
    $f'(x) = -32t$\\
    $f'(5) = -160 ft.s^{-1}$\\

    $f(x)$ is continuous at $x_0$ if
    \[ lim_{x \to x_0}; f(x) = f(x_0)  \Leftrightarrow \lim_{x \to x_0}; f(x) - f(x_0) = 0\]
    \textbf{Theorem :}
    If $f$ is differentiable at $x_0$ then $f$ is continuous at $x_0$
    \[\lim_{x \to x_0}; f(x) - f(x_0) = \lim_{x \to x_0};\frac{f(x) - f(x_0)}{x-x_0}(x-x_0) = f'(x_0).0 = 0 \]

    \paragraph{Derivatives of composed functions}

    \begin{align*} (u+v)'(x) &= \lim_{\Delta x \to 0}; \frac{(u+v)(x+\Delta x) - (u +v)(x)}{\Delta x}\\
        &= \lim_{\Delta x \to 0}; \frac{u(x+\Delta x) + v(x+\Delta x) - u(x) - v(x)}{\Delta x}\\
        &= u'(x) + v'(x)
    \end{align*}

    \begin{align*}
        (uv)' &= u'v + v'u\\
        (\frac{u}{v})' &= \frac{u'v - v'u}{v^2}
    \end{align*}


    \[ \lim_{x \to 0}; \frac{\sin x}{x} = 1\]
    \[    \lim_{x \to 0}; \frac{\cos x -1}{x} = 0\]

    \begin{align*}
        f'(x) &= \frac{d}{dx} \sin x\\
        &= \lim_{x+\Delta x} \frac{\sin(x+\Delta x) - \sin x}{\Delta x}\\
        &= \lim_{x+\Delta x} \frac{\sin x \cos \Delta x + \sin \Delta x \cos x - \sin x}{\Delta x}\\
        &= \lim_{x+\Delta x} \frac{\sin(\cos \Delta x -1)}{\Delta x} + \lim_{x+\Delta x} \frac{\cos x \sin \Delta x}{\Delta x}\\
        &= 0 + \cos x
    \end{align*}

    \paragraph{Chain rules}
    $ y= f(g(t))$\\
    \[ \frac{dy}{dt} = \frac{dy}{dx}\frac{dx}{dx} \]

    $y = f(x) = \sin x$\\
    $x = g(t) = t^2$\\
    $y = sin(t^2)$\\
    \[ \frac{d}{dt}(\sin t^2) = (\frac{dy}{dx})(\frac{dx}{dt})=(\cos x)(2t) = \cos(t^2)2t \]
    $f(g(x))' = g'(x)f'(g(x))$

    \paragraph{Implicit differntiation}

    $y = f(x) $\\
    $x^2 + y^2 = 1 $\\


    \begin{align*}
        \frac{d}{dx} (x^a) &= ax^{a-1}\\
        a &= m/n ; y = x^{m/n} ; y^n = x^m\\
        ny^{n-1}.\frac{dy}{dx} &= mx^{m-1}\\
        \frac{dy}{dx} &= \frac{m}{n} \frac{x^{m-1}}{y^{n-1}}\\
        &= \frac{m}{n} \frac{x^{m-1}}{x^{{m-1}^{n-1}}}\\
        &= \frac{m}{n} \frac{x^{m-1}}{x^{\frac{m(n-1)}{n}}}\\
        \frac{m}{n}x^{\frac{m}{n} -1} &= ax^{a-1}
    \end{align*}

    \begin{center}
        $\cos a + b = \sin a \cos b + \cos a \sin b$
        $\sin a+b = \cos a \cos b + \sin a \sin b$
    \end{center}

    We can note derivative with $D^n$ with $n$ the degree of the derivative.\\
    $D^2 x^n = n(n-1)x^{n-2}$ so generalizing :
    \begin{align*}
        D^{n-1} x^n &= n(n-1)...2 x^{n-(n-1)}\\
        &= n! x
    \end{align*}

    For a bacterial populaiton, $y_0$ is the initial site of the population, $t$ is the time in days. The bact√©rias double every days.\\
    $y(t) = 2^t y_0$\\~\\

    $A_0$ is the inital amount, $n$ the number of years, the interest rate is $5\%$.\\
    $A(n) = A_0 (1.05)^n$\\

    \begin{align*}
        \frac{d}{dx} a^x &= \lim {\Delta x \to 0} ; \frac{a^{x+\Delta x} - a^x}{\Delta x}\\
        &= \lim {\Delta x \to 0} ; \frac{a^x (a^{\Delta x} -1)}{\Delta x}\\
        &= a^x \lim {\Delta x \to 0} ; \frac{a^{\Delta x} -1}{\Delta x}\\
        with \frac{d}{dx} a^x = a^x M(a)\\
        \frac{d}{dx}a^x_{x=0} &= a^0 M(a) = M(a)\\
        So :
        \frac{d}{dx} e^x &= e^x
    \end{align*}
    $f(x) = 2^x$ initial function for wich we want to comute the derivative.\\
    $f(kx) = 2^{kx} = (2^k)^x = b^x$ (with $b=2^k$)\\
    So $\frac{d}{dx}b^x = kf'(kx)$
    \[ \frac{d}{dx}b^x_{x=0} = kf'(0) = M(2)k \]
    If $y=e^x$ then $\ln y = x$\\

    \begin{align*}
        \frac{d}{dx} \ln x\\
        w = \ln x \Rightarrow e^w = x\\
        \frac{d}{dx} e^w &= \frac{d}{dx} x = 1\\
        \frac{d}{dx} e^w \frac{dw}{dx} &= 1\\
        e^w \frac{dw}{dx} &= 1 \Rightarrow \\
        \frac{dw}{dx} &= \frac{1}{e^w} = \frac{1}{x}
    \end{align*}

    \begin{align*}
        \frac{d}{dx} a^x &= ?\\
        a^x &= (e^{\ln a})^x = e^{x\ln a}\\
        \frac{d}{dx} a^x &= e^{x\ln a} . \ln a\\
        &= a^x \ln a\\
        M(a) &= \ln a
    \end{align*}

    \begin{align*}
        \frac{d}{dx} u &= ?\\
        \frac{d}{dx} \ln u &= \frac{d \ln u}{du} . \frac{du}{dx} \\
        &= \frac{1}{u}.\frac{du}{dx}\\
        \frac{d}{dx} a^x = ? , u = a^x , \ln u = x\ln a \\
        (\ln u)' &= \ln a. \frac{u'}{u}\\
        &= \ln a . u'\\
        &= \ln a .u \\
        (a^x)' &= a^x \ln a
    \end{align*}

    \subsection{Differential equations}

    \subsection{Antiderivatives}
    \label{sub:Antiderivatives}

    $\int G(x)= g(x)dx $ and $G'(x)=g(x)$\\

    \begin{align*}
        \int \sin x dx &= \cos x + C\\
        Find G(x) such as G'(x)= \sin x
    \end{align*}

    \begin{align*}
        \int x^a dx &= \frac{x^{a+1}}{a+1}+C\\
        (\frac{x^{a+1}}{a+1}+C)' &= \frac{1}{a+1}.(a+1).x^a + 0\\
        &= x^a\\
        ~\\
        If a = -1, x^a = x^{-1} = \frac{1}{x}\\
        \int \frac{dx}{x} &= \ln |x| + C\\
        (\ln(-x))' &= \frac{1}{-x}.(-1)\\
        &= \frac{1}{x}
    \end{align*}

    \textit{Theorem : } If $F' = G'$, then $F(x)=G(x)+C$ for all $x$.\\
    \textit{Proof :} If $F' = G'$, then $(F - G)' = F' - G' = 0$\\
    Hence, $F(x)-G(x)$ is a constant. Derivative is 0 $\rightarrow$ function is constant (follows from the mean value theorem).\\

    \[
    \label{Mean value theorem}
    \frac{f(b) - f(a)}{b-a} = f'(c)~ ~ ~ ~
    f ~differentiable ~for~ a~ < ~x ~< ~b ~ ~ ~ ~
    f ~continuous ~for~ a \leq x \leq b
    \]

    \begin{align*}
        \int x^3 (x^4 + 2)^5 dx &= \\
        with~ u = x^4 +2 ~and ~du = 4x^3 dx
        &= \int \frac{u^5}{4}du\\
        &= \frac{1}{4}.\frac{1}{6}u^6+C\\
        &= \frac{u^6}{24}+C\\
        &= \frac{(x^4 +2)^6}{24}+C
    \end{align*}

    \textit{Example}
    \begin{align*}
        \int frac{dx}{x\ln x} &= \int \frac{du}{u}\\
        &= \ln |u| + C\\
        &= \ln |\ln x| +C\\
        with~ u=\ln x, ~ du=\frac{1}{x}dx
    \end{align*}


    %% Graph with exponential, logarithm.

    \subsubsection{Differential equations}

    $\frac{dy}{dx} = f(x)$\\
    $y = \int f(x)dx$\\

    \textit{Example :}\\
    \begin{align*}
        \frac{d}{dy}y + xy &= 0 \\
        \Leftrightarrow \frac{dy}{dx}&=-xy\\
        \Rightarrow \frac{dy}{y} &= -xdx\\
        \int \frac{dy}{y} &= -\int xdx \\
        \ln |y| &= - \frac{x^2}{2}+C\\
        |y| &= e^{-\frac{x^2}{2}+C} \\
        &= e^{-\frac{x^2}{2}}.A ~ with ~ A=e^C
    \end{align*}

    \textit{Generalisation :}
    \begin{align*}
        \frac{dy}{dx} &= f(x)g(y)\\
        \frac{dy}{g(y)} &= f(x)dx\\
        H(y) &= F(x) +C \\
        y &= H^{-1}(F(x)+C)
    \end{align*}



    \subsection{Linear Algebra}

\end{document}
